############
# author: Kent O'Sullivan
# purpose: The privacy namespace is a stub designed to allow for the development of an IoT ontology.
# Last Updated: 16 Feb 22
############

@prefix privacy: <https://github.com/osullik/IoT-Privacy/blob/main/privacy.ttl>.
@prefix sense: <https://github.com/osullik/IoT-Privacy/blob/main/senses.ttl>.
@prefix social_IOT_KB: <https://github.com/osullik/IoT-Privacy/blob/main/social_IOT_KB.ttl>.

@prefix rdf:    	<http://www.w3.org/1999/02/22-rdf-syntax-ns#> .
@prefix xsd:     	<http://www.w3.org/2001/XMLSchema#> .
@prefix rdfs:    	<http://www.w3.org/2000/01/rdf-schema#> .
@prefix owl:		<http://www.w3.org/2002/07/owl#> .


#     ____   _          _      ____    ____    _____   ____  
#    / ___| | |        / \    / ___|  / ___|  | ____| / ___| 
#   | |     | |       / _ \   \___ \  \___ \  |  _|   \___ \ 
#   | |___  | |___   / ___ \   ___) |  ___) | | |___   ___) |
#    \____| |_____| /_/   \_\ |____/  |____/  |_____| |____/ 
#                                                            

### The Following Seven Classes are derived from Finn's Privacy model. 
### Ref: Rachel L Finn, David Wright, and Michael Friedewald. “Seven types of privacy”. In: European data protection: coming of age. Springer, 2013, pp. 3– 32.

privacy:PrivacyType
	rdf:type rdfs:Class ;
	rdfs:comment "Parent class for the seven types of privacy from Finn's model"^^xsd:string ;
	rdfs:label "Privacy Type"^^xsd:string .

privacy:PersonalPrivacy
	rdf:type rdfs:Class ;
	rdfs:comment "Privacy of the person encompasses the right to keep body functions and body characteristics (such as genetic codes and biometrics) private."^^xsd:string ;
	rdfs:label "Privacy of the Person"^^xsd:string ;
	rdfs:subClassOf privacy:PrivacyType.

privacy:BehaviourAndActionPrivacy
	rdf:type rdfs:Class ;
	rdfs:comment "The ability to behave in public, semi-public or one’s private space without having actions monitored or controlled by others con- tributes to the development and exercise of autonomy and freedom in thought and action."^^xsd:string ;
	rdfs:label "Privacy of Behaviour and Action"^^xsd:string ;
	rdfs:subClassOf privacy:PrivacyType.

privacy:CommunicationPrivacy
rdf:type rdfs:Class ; 
	rdfs:comment "Privacy of communication aims to avoid the interception of communications, including mail interception, the use of bugs, directional microphones, telephone or wireless communication interception or recording and access to e-mail messages."^^xsd:string ;
	rdfs:label "Privacy of Communications"^^xsd:string ;
	rdfs:subClassOf privacy:PrivacyType.

privacy:DataAndImagePrivacy
rdf:type rdfs:Class ;
	rdfs:comment "privacy of data and image includes concerns about making sure that individuals’ data is not automatically available to other individuals and organisations and that people can exercise a substantial degree of control over that data and its use"^^xsd:string ;
	rdfs:label "Privacy of Data and Image"^^xsd:string ;
	rdfs:subClassOf privacy:PrivacyType.

privacy:ThoughtAndFeelingPrivacy
rdf:type rdfs:Class ;
	rdfs:comment "People have a right not to share their thoughts or feelings or to have those thoughts or feeling revealed. Individuals should have the right to think whatever they like. Privacy of thought and feelings can be distinguished from privacy of the person, in the same way that the mind can be distinguished from the body."^^xsd:string ;
	rdfs:label "Privacy of Thought and Feeling"^^xsd:string ;
	rdfs:subClassOf privacy:PrivacyType.

privacy:LocationAndSpacePrivacy
rdf:type rdfs:Class ;
	rdfs:comment "individuals have the right to move about in public or semi-public space without being identified, tracked or monitored. This conception of privacy also includes a right to solitude and a right to privacy in spaces such as the home, the car or the office."^^xsd:string ;
	rdfs:label "Privacy of Location and Space"^^xsd:string ;
	rdfs:subClassOf privacy:PrivacyType.

privacy:AssociationPrivacy
rdf:type rdfs:Class ;
	rdfs:comment "Privacy of Association (including group privacy) is concerned with people’s right to associate with whomever they wish, without being monitored. "^^xsd:string ;
	rdfs:label "Privacy of Association"^^xsd:string ;
	rdfs:subClassOf privacy:PrivacyType.


### The following class reprsents the person being threatened, or in this case "Persona"

privacy:Persona
	rdf:type rdfs:Class ;
	rdfs:comment "Parent class for the five sensory dimensions" ;
	rdfs:label "Persona".


#    ____    ____     ___    ____    _____   ____    _____   ___   _____   ____  
#   |  _ \  |  _ \   / _ \  |  _ \  | ____| |  _ \  |_   _| |_ _| | ____| / ___| 
#   | |_) | | |_) | | | | | | |_) | |  _|   | |_) |   | |    | |  |  _|   \___ \ 
#   |  __/  |  _ <  | |_| | |  __/  | |___  |  _ <    | |    | |  | |___   ___) |
#   |_|     |_| \_\  \___/  |_|     |_____| |_| \_\   |_|   |___| |_____| |____/ 
#    

### The following properties relate to describing the "Persona" entity. 
privacy:personaID
	rdf:type rdf:Property ; 
	rdfs:comment "The unique identification number of a persona, derived from their digital persona. Could be a MAC Address, AdvertisingID etc"^^xsd:string ;
	rdfs:label "Persona ID"^^xsd:string ;
	rdfs:domain privacy:Persona ;
	rdfs:range xsd:string .

privacy:personaName
	rdf:type rdf:Property ; 
	rdfs:comment "The 'true name' of an individual persona"^^xsd:string ;
	rdfs:label "Persona Name"^^xsd:string ;
	rdfs:domain privacy:Persona ;
	rdfs:range xsd:string .

privacy:exposesIdentity
	rdf:type rdf:Property ;
	rdfs:comment "The ability to determine WHO an individual is"^^xsd:string ;
	rdfs:label "Exposes Identity (WHO)" ;
	rdfs:domain privacy:Persona ;
	rdfs:range xsd:boolean .

privacy:exposesAction
	rdf:type rdf:Property ;
	rdfs:comment "The ability to determine WHAT an individual has done"^^xsd:string ;
	rdfs:label "Exposes Action (WHAT)" ;
	rdfs:domain privacy:Persona ;
	rdfs:range xsd:boolean .

privacy:exposesTime 
	rdf:type rdf:Property ;
	rdfs:comment "The ability to determine WHEN something occurs"^^xsd:string ;
	rdfs:label "Exposes Time (WHEN)" ;
	rdfs:domain privacy:Persona ;
	rdfs:range xsd:boolean .

privacy:exposesLocation
	rdf:type rdf:Property ;
	rdfs:comment "The ability to determine WHERE an individual is"^^xsd:string ;
	rdfs:label "Exposes Location (WHERE)" ;
	rdfs:domain privacy:Persona ;
	rdfs:range xsd:boolean .

privacy:exposesMotive
	rdf:type rdf:Property ;
	rdfs:comment "The ability to determine WHY an individual does something. Here generally can only be determined if the confidentiality of their communications is breached, as someone telling someone else their motive is the closest that we are likely to get to understanding it"^^xsd:string ;
	rdfs:label "Exposes Motive (WHY)" ;
	rdfs:domain privacy:Persona ;
	rdfs:range xsd:boolean .


#    ____    _____   _          _      _____   ___    ___    _   _   ____    _   _   ___   ____    ____  
#   |  _ \  | ____| | |        / \    |_   _| |_ _|  / _ \  | \ | | / ___|  | | | | |_ _| |  _ \  / ___| 
#   | |_) | |  _|   | |       / _ \     | |    | |  | | | | |  \| | \___ \  | |_| |  | |  | |_) | \___ \ 
#   |  _ <  | |___  | |___   / ___ \    | |    | |  | |_| | | |\  |  ___) | |  _  |  | |  |  __/   ___) |
#   |_| \_\ |_____| |_____| /_/   \_\   |_|   |___|  \___/  |_| \_| |____/  |_| |_| |___| |_|     |____/ 
#                                   

### The Following Relationships define the link from the interrogative dimension to the privacy type. 

privacy:threatens
	rdf:type rdfs:Property ; 
	rdfs:comment "Parent class for all privacy risks"^^xsd:string ;
	rdfs:label "What threatens the privacy type" ; 
	rdfs:domain privacy:Persona ; 
	rdfs:range privacy:PrivacyType .
